rupicola/io/Compilation.fst
@@ -47,186 +47,186 @@ and compile_oprod #g #a (#s:fs_oprod g a) (qs:oprod_quotation g s) : Tot exp (de
 let rec lem_compile_superset #g (#a:qType) (#s:fs_oval g a) (qs:g ⊢ s)
   : Lemma (ensures (s ⊐ (compile qs))) (decreases qs)
   = match qs with
-  | Qtt -> C1.equiv_oval_unit g
-  | QVar0 #g' #_ -> C1.equiv_oval_var0 g' a
+  | Qtt -> C1.compat_oval_unit g
+  | QVar0 #g' #_ -> C1.compat_oval_var0 g' a
   | QVarS #g' #_ #b #x qx ->
     lem_compile_superset qx;
-    C1.equiv_varS #g' #a #b x (compile qx)
-  | QFd fd -> C1.equiv_oval_file_descr g fd
-  | QAppGhost -> C1.equiv_oval_unit g
+    C1.compat_varS #g' #a #b x (compile qx)
+  | QFd fd -> C1.compat_oval_file_descr g fd
+  | QAppGhost -> C1.compat_oval_unit g
   | QApp #_ #qa #qb #f #x qf qx ->
     lem_compile_superset qf;
     lem_compile_superset qx;
-    C1.equiv_oval_app f x (compile qf) (compile qx)
+    C1.compat_oval_app f x (compile qf) (compile qx)
   | QLambda #_ #_ #_ #body qbody ->
     lem_compile_superset qbody;
-    C1.equiv_oval_lambda body (compile qbody)
-  | QFalse -> C1.equiv_oval_false g
-  | QTrue -> C1.equiv_oval_true g
-  | QStringLit #_ str -> C1.equiv_oval_string g str
+    C1.compat_oval_lambda body (compile qbody)
+  | QFalse -> C1.compat_oval_false g
+  | QTrue -> C1.compat_oval_true g
+  | QStringLit #_ str -> C1.compat_oval_string g str
   | QStringEq #_ #s1 qs1 #s2 qs2 ->
     lem_compile_superset qs1;
     lem_compile_superset qs2;
-    C1.equiv_oval_string_eq s1 s2 (compile qs1) (compile qs2)
+    C1.compat_oval_string_eq s1 s2 (compile qs1) (compile qs2)
   | QIf #_ #_ #c qc #t qt #e qe ->
     lem_compile_superset qc;
     lem_compile_superset qt;
     lem_compile_superset qe;
-    C1.equiv_oval_if c t e (compile qc) (compile qt) (compile qe)
+    C1.compat_oval_if c t e (compile qc) (compile qt) (compile qe)
   | QMkpair #_ #a1 #a2 #s1 #s2 q1 q2 ->
     lem_compile_superset q1;
     lem_compile_superset q2;
-    C1.equiv_oval_pair s1 s2 (compile q1) (compile q2)
+    C1.compat_oval_pair s1 s2 (compile q1) (compile q2)
   | QFst #_ #_ #_ #p qp ->
     lem_compile_superset qp;
-    C1.equiv_oval_pair_fst p (compile qp)
+    C1.compat_oval_pair_fst p (compile qp)
   | QSnd #_ #_ #_ #p qp ->
     lem_compile_superset qp;
-    C1.equiv_oval_pair_snd p (compile qp)
+    C1.compat_oval_pair_snd p (compile qp)
   | QInl #_ #_ #t2 #p qp ->
     lem_compile_superset qp;
-    C1.equiv_oval_inl t2 p (compile qp)
+    C1.compat_oval_inl t2 p (compile qp)
   | QInr #_ #t1 #_ #p qp ->
     lem_compile_superset qp;
-    C1.equiv_oval_inr t1 p (compile qp)
+    C1.compat_oval_inr t1 p (compile qp)
   | QCase #_ #_ #_ #_ #cond qcond #inlc qinlc #inrc qinrc ->
     lem_compile_superset qcond;
     lem_compile_superset qinlc;
     lem_compile_superset qinrc;
-    C1.equiv_oval_case cond inlc inrc (compile qcond) (compile qinlc) (compile qinrc)
+    C1.compat_oval_case cond inlc inrc (compile qcond) (compile qinlc) (compile qinrc)
   | QLambdaProd #_ #_ #_ #body qbody ->
     lem_compile_superset_prod qbody;
-    C1.equiv_oval_lambda_oprod body (compile_oprod qbody)
+    C1.compat_oval_lambda_oprod body (compile_oprod qbody)
 and lem_compile_superset_prod #g (#a:qType) (#s:fs_oprod g a) (qs:oprod_quotation g s)
   : Lemma (ensures (s ⊒ (compile_oprod qs))) (decreases qs)
   =
   match qs with
   | QOpenfile #_ #fnm qfnm ->
     lem_compile_superset qfnm;
-    C1.equiv_oprod_openfile_oval fnm (compile qfnm)
+    C1.compat_oprod_openfile_oval fnm (compile qfnm)
   | QRead #_ #fd qfd ->
     lem_compile_superset qfd;
-    C1.equiv_oprod_read_oval fd (compile qfd)
+    C1.compat_oprod_read_oval fd (compile qfd)
   | QWrite #_ #fd #msg qfd qmsg ->
     lem_compile_superset qfd;
     lem_compile_superset qmsg;
-    C1.equiv_oprod_write_oval fd msg (compile qfd) (compile qmsg)
+    C1.compat_oprod_write_oval fd msg (compile qfd) (compile qmsg)
   | QClose #_ #fd qfd ->
     lem_compile_superset qfd;
-    C1.equiv_oprod_close_oval fd (compile qfd)
+    C1.compat_oprod_close_oval fd (compile qfd)
   | QReturn #_ #_ #x qx ->
     lem_compile_superset qx;
-    C1.equiv_oprod_return x (compile qx)
+    C1.compat_oprod_return x (compile qx)
   | QBindProd #_ #_ #_ #m #k qm qk ->
     lem_compile_superset_prod qm;
     lem_compile_superset_prod qk;
-    C1.equiv_oprod_bind m k (compile_oprod qm) (compile_oprod qk)
+    C1.compat_oprod_bind m k (compile_oprod qm) (compile_oprod qk)
   | QAppProd #_ #_ #_ #f #x qf qx ->
     lem_compile_superset qf;
     lem_compile_superset qx;
-    C1.equiv_oprod_app_oval_oval f x (compile qf) (compile qx)
+    C1.compat_oprod_app_oval_oval f x (compile qf) (compile qx)
   | QIfProd #_ #_ #c qc #t qt #e qe ->
     lem_compile_superset qc;
     lem_compile_superset_prod qt;
     lem_compile_superset_prod qe;
-    C1.equiv_oprod_if_oval c t e (compile qc) (compile_oprod qt) (compile_oprod qe)
+    C1.compat_oprod_if_oval c t e (compile qc) (compile_oprod qt) (compile_oprod qe)
   | QCaseProd #_ #_ #_ #_ #cond qcond #inlc qinlc #inrc qinrc ->
     lem_compile_superset qcond;
     lem_compile_superset_prod qinlc;
     lem_compile_superset_prod qinrc;
-    C1.equiv_oprod_case_oval cond inlc inrc (compile qcond) (compile_oprod qinlc) (compile_oprod qinrc)
+    C1.compat_oprod_case_oval cond inlc inrc (compile qcond) (compile_oprod qinlc) (compile_oprod qinrc)
 
 let rec lem_compile_subset #g (#a:qType) (#s:fs_oval g a) (qs:g ⊢ s)
   : Lemma (ensures (s ⊏ (compile qs))) (decreases qs)
   = match qs with
-  | Qtt -> C2.equiv_oval_unit g
-  | QVar0 #g' #_ -> C2.equiv_oval_var0 g' a
+  | Qtt -> C2.compat_oval_unit g
+  | QVar0 #g' #_ -> C2.compat_oval_var0 g' a
   | QVarS #g' #_ #b #x qx ->
     lem_compile_subset qx;
-    C2.equiv_varS #g' #a #b x (compile qx)
-  | QFd fd -> C2.equiv_oval_file_descr g fd
-  | QAppGhost -> C2.equiv_oval_unit g
+    C2.compat_varS #g' #a #b x (compile qx)
+  | QFd fd -> C2.compat_oval_file_descr g fd
+  | QAppGhost -> C2.compat_oval_unit g
   | QApp #_ #qa #qb #f #x qf qx ->
     lem_compile_subset qf;
     lem_compile_subset qx;
-    C2.equiv_oval_app f x (compile qf) (compile qx)
+    C2.compat_oval_app f x (compile qf) (compile qx)
   | QLambda #_ #_ #_ #body qbody ->
     lem_compile_subset qbody;
-    C2.equiv_oval_lambda body (compile qbody)
-  | QFalse -> C2.equiv_oval_false g
-  | QTrue -> C2.equiv_oval_true g
-  | QStringLit #_ str -> C2.equiv_oval_string g str
+    C2.compat_oval_lambda body (compile qbody)
+  | QFalse -> C2.compat_oval_false g
+  | QTrue -> C2.compat_oval_true g
+  | QStringLit #_ str -> C2.compat_oval_string g str
   | QStringEq #_ #s1 qs1 #s2 qs2 ->
     lem_compile_subset qs1;
     lem_compile_subset qs2;
-    C2.equiv_oval_string_eq s1 s2 (compile qs1) (compile qs2)
+    C2.compat_oval_string_eq s1 s2 (compile qs1) (compile qs2)
   | QIf #_ #_ #c qc #t qt #e qe ->
     lem_compile_subset qc;
     lem_compile_subset qt;
     lem_compile_subset qe;
-    C2.equiv_oval_if c t e (compile qc) (compile qt) (compile qe)
+    C2.compat_oval_if c t e (compile qc) (compile qt) (compile qe)
   | QMkpair #_ #a1 #a2 #s1 #s2 q1 q2 ->
     lem_compile_subset q1;
     lem_compile_subset q2;
-    C2.equiv_oval_pair s1 s2 (compile q1) (compile q2)
+    C2.compat_oval_pair s1 s2 (compile q1) (compile q2)
   | QFst #_ #_ #_ #p qp ->
     lem_compile_subset qp;
-    C2.equiv_oval_pair_fst p (compile qp)
+    C2.compat_oval_pair_fst p (compile qp)
   | QSnd #_ #_ #_ #p qp ->
     lem_compile_subset qp;
-    C2.equiv_oval_pair_snd p (compile qp)
+    C2.compat_oval_pair_snd p (compile qp)
   | QInl #_ #_ #t2 #p qp ->
     lem_compile_subset qp;
-    C2.equiv_oval_inl t2 p (compile qp)
+    C2.compat_oval_inl t2 p (compile qp)
   | QInr #_ #t1 #_ #p qp ->
     lem_compile_subset qp;
-    C2.equiv_oval_inr t1 p (compile qp)
+    C2.compat_oval_inr t1 p (compile qp)
   | QCase #_ #_ #_ #_ #cond qcond #inlc qinlc #inrc qinrc ->
     lem_compile_subset qcond;
     lem_compile_subset qinlc;
     lem_compile_subset qinrc;
-    C2.equiv_oval_case cond inlc inrc (compile qcond) (compile qinlc) (compile qinrc)
+    C2.compat_oval_case cond inlc inrc (compile qcond) (compile qinlc) (compile qinrc)
   | QLambdaProd #_ #_ #_ #body qbody ->
     lem_compile_subset_prod qbody;
-    C2.equiv_oval_lambda_oprod body (compile_oprod qbody)
+    C2.compat_oval_lambda_oprod body (compile_oprod qbody)
 and lem_compile_subset_prod #g (#a:qType) (#s:fs_oprod g a) (qs:oprod_quotation g s)
   : Lemma (ensures (s ⊑ (compile_oprod qs))) (decreases qs)
   =
   match qs with
   | QOpenfile #_ #fnm qfnm ->
     lem_compile_subset qfnm;
-    C2.equiv_oprod_openfile_oval fnm (compile qfnm)
+    C2.compat_oprod_openfile_oval fnm (compile qfnm)
   | QRead #_ #fd qfd ->
     lem_compile_subset qfd;
-    C2.equiv_oprod_read_oval fd (compile qfd)
+    C2.compat_oprod_read_oval fd (compile qfd)
   | QWrite #_ #fd #msg qfd qmsg ->
     lem_compile_subset qfd;
     lem_compile_subset qmsg;
-    C2.equiv_oprod_write_oval fd msg (compile qfd) (compile qmsg)
+    C2.compat_oprod_write_oval fd msg (compile qfd) (compile qmsg)
   | QClose #_ #fd qfd ->
     lem_compile_subset qfd;
-    C2.equiv_oprod_close_oval fd (compile qfd)
+    C2.compat_oprod_close_oval fd (compile qfd)
   | QReturn #_ #_ #x qx ->
     lem_compile_subset qx;
-    C2.equiv_oprod_return x (compile qx)
+    C2.compat_oprod_return x (compile qx)
   | QBindProd #_ #_ #_ #m #k qm qk ->
     lem_compile_subset_prod qm;
     lem_compile_subset_prod qk;
-    C2.equiv_oprod_bind m k (compile_oprod qm) (compile_oprod qk)
+    C2.compat_oprod_bind m k (compile_oprod qm) (compile_oprod qk)
   | QAppProd #_ #_ #_ #f #x qf qx ->
     lem_compile_subset qf;
     lem_compile_subset qx;
-    C2.equiv_oprod_app_oval_oval f x (compile qf) (compile qx)
+    C2.compat_oprod_app_oval_oval f x (compile qf) (compile qx)
   | QIfProd #_ #_ #c qc #t qt #e qe ->
     lem_compile_subset qc;
     lem_compile_subset_prod qt;
     lem_compile_subset_prod qe;
-    C2.equiv_oprod_if_oval c t e (compile qc) (compile_oprod qt) (compile_oprod qe)
+    C2.compat_oprod_if_oval c t e (compile qc) (compile_oprod qt) (compile_oprod qe)
   | QCaseProd #_ #_ #_ #_ #cond qcond #inlc qinlc #inrc qinrc ->
     lem_compile_subset qcond;
     lem_compile_subset_prod qinlc;
     lem_compile_subset_prod qinrc;
-    C2.equiv_oprod_case_oval cond inlc inrc (compile qcond) (compile_oprod qinlc) (compile_oprod qinrc)
+    C2.compat_oprod_case_oval cond inlc inrc (compile qcond) (compile_oprod qinlc) (compile_oprod qinrc)
 
 let rec lem_compile_fv_in_env #g (#a:qType) (#s:fs_oval g a) (qs:g ⊢ s)
   : Lemma (ensures fv_in_env g (compile qs)) (decreases qs)
